Examples/Scroll/Keccak/Lookups.lean
@@ -1,9 +1,0 @@
-import Examples.Scroll.Keccak.Extraction
-
-namespace Keccak
-
-  namespace Lookups
-    def normalize_3 (c: ValidCircuit P P_Prime) (row: ℕ) := (c.get_fixed 8 row, c.get_fixed 9 row)
-  end Lookups
-
-end Keccak
