Examples/Scroll/Keccak/All.lean
@@ -4,6 +4,6 @@ import Examples.Scroll.Keccak.Attributes
 import Examples.Scroll.Keccak.CellManager
 import Examples.Scroll.Keccak.Constants
 import Examples.Scroll.Keccak.Extraction
-import Examples.Scroll.Keccak.Lookups
+import Examples.Scroll.Keccak.Lookups.All
 import Examples.Scroll.Keccak.Selectors
 import Examples.Scroll.Keccak.Util
