Examples/Scroll/Keccak/Lookups/All.lean
@@ -1,0 +1,2 @@
+import Examples.Scroll.Keccak.Lookups.Columns
+import Examples.Scroll.Keccak.Lookups.Normalize_3
